examples/rv: Give more readable names to registers

examples/rv/RVCore.v
@@ -706,6 +706,43 @@ Module  RV32ICore.
     | _ => false
     end.
 
+  Definition rv_register_name (v: Vect.index 32) :=
+    match index_to_nat v with
+    | 0  => "x00_zero" (* hardwired zero *)
+    | 1  => "x01_ra" (* caller-saved, return address *)
+    | 2  => "x02_sp" (* callee-saved, stack pointer *)
+    | 3  => "x03_gp" (* global pointer *)
+    | 4  => "x04_tp" (* thread pointer *)
+    | 5  => "x05_t0" (* caller-saved, temporary registers *)
+    | 6  => "x06_t1" (* caller-saved, temporary registers *)
+    | 7  => "x07_t2" (* caller-saved, temporary registers *)
+    | 8  => "x08_s0_fp" (* callee-saved, saved register / frame pointer *)
+    | 9  => "x09_s1" (* callee-saved, saved register *)
+    | 10 => "x10_a0" (* caller-saved, function arguments / return values *)
+    | 11 => "x11_a1" (* caller-saved, function arguments / return values *)
+    | 12 => "x12_a2" (* caller-saved, function arguments *)
+    | 13 => "x13_a3" (* caller-saved, function arguments *)
+    | 14 => "x14_a4" (* caller-saved, function arguments *)
+    | 15 => "x15_a5" (* caller-saved, function arguments *)
+    | 16 => "x16_a6" (* caller-saved, function arguments *)
+    | 17 => "x17_a7" (* caller-saved, function arguments *)
+    | 18 => "x18_s2" (* callee-saved, saved registers *)
+    | 19 => "x19_s3" (* callee-saved, saved registers *)
+    | 20 => "x20_s4" (* callee-saved, saved registers *)
+    | 21 => "x21_s5" (* callee-saved, saved registers *)
+    | 22 => "x22_s6" (* callee-saved, saved registers *)
+    | 23 => "x23_s7" (* callee-saved, saved registers *)
+    | 24 => "x24_s8" (* callee-saved, saved registers *)
+    | 25 => "x25_s9" (* callee-saved, saved registers *)
+    | 26 => "x26_s10" (* callee-saved, saved registers *)
+    | 27 => "x27_s11" (* callee-saved, saved registers *)
+    | 28 => "x28_t3" (* caller-saved, temporary registers *)
+    | 29 => "x29_t4" (* caller-saved, temporary registers *)
+    | 30 => "x30_t5" (* caller-saved, temporary registers *)
+    | 31 => "x31_t6" (* caller-saved, temporary registers *)
+    | _ => ""
+    end.
+
   Instance FiniteType_toIMem : FiniteType MemReq.reg_t := _.
   Instance FiniteType_fromIMem : FiniteType MemResp.reg_t := _.
   Instance FiniteType_toDMem : FiniteType MemReq.reg_t := _.
